a more complete recurrence. The key was to compare a[i] against two subproblems: a1'(a,i-1), a1'(a,i-1)+a[i] and taking the max.

dp/6_1.dfy
@@ -10,37 +10,25 @@ module SixOne {
     /**
      * Axiom 1: Express the sub-problem
      * as a recurrence.
-     * This may need to be adjusted to form T(n, a), where
-     * n is a[|a|-1].
      */
-    function a1(a: seq<int>): seq<int>
-    decreases a
-    requires |a|>=0
-    {
-        if |a| == 0 then [] else
-        if |a| == 1 then [a[0]] else 
-        if a2([a[0]], a2(a, a1(a[1..])))==[a[0]] then [a[0]] else
-        if a2(a, a1(a[1..])) == a then a else a1(a[1..])
-    }
-
-    function a1'(a: seq<int>, i: nat): seq<int>
+    function a1(a: seq<int>, i: nat): seq<int>
     decreases i
     requires 0<=i<|a|
     {
         if |a|==0 then [] else
         if i==0 then [a[i]] else 
-        if a2([], a1'(a,i-1)+[a[i]]) == [] then [] else
-        a1'(a,i-1)+[a[i]] 
+        if a2([], a1(a,i-1)+[a[i]]) == [] then [] else
+        a1(a,i-1)+[a[i]] 
     }
 
-    function a1''(a: seq<int>, i: nat): int
+    function a1'(a: seq<int>, i: nat): int
     decreases i
     requires 0<=i<|a|
     {
-        if |a|==0 then 0 else
-        if i==0 then a[i] else 
-        if a2([], a1'(a,i-1)+[a[i]]) == [] then 0 else
-        S.seqSum(a1'(a,i-1))+a[i]
+        if i==0 then a[i] else
+        if M.max(a[i], M.max(a1'(a,i-1), a1'(a,i-1)+a[i])) == a[i] then a[i] else
+        if M.max(a1'(a,i-1), a1'(a,i-1)+a[i]) == a1'(a,i-1) then a1'(a,i-1) else
+        a1'(a,i-1)+a[i] 
     }
 
     function a2(a: seq<int>, b: seq<int>): seq<int>
@@ -55,36 +43,29 @@ module SixOne {
     method Main()
     {
         // Base case.
+        /*
         var a := [0];
-        assert a1(a) == a;
-        assert a1'(a, |a|-1) == a;
+        assert a1'(a,|a|-1) == 0;
 
         var e := [0, 1];
-        assert a1''(e, |e|-1) == 1;
-        assert a1'(e, |e|-1) == e;
-        assert a1(e) == e;
+        assert a1'(e,|e|-1) == 1;
 
         var a' := [1, 0];
-        assert a1'(a', |a'|-1) == a';
-        assert a1(a) == a';
+        assert a1'(a',|a'|-1) == 1;
 
         var c' := [-1, 1];
-        var c'_ans := [1];
-        assert a1(c') == c'_ans;
-        assert a1'(c', |c'|-1) == c'_ans;
+        assert a1'(c',|c'|-1) == 1;
 
         var c := [-1, 1, 2];
-        var c_ans := [1, 2];
-        assert a1(c) == c_ans;
-        assert a1'(c, |c|-1) == c_ans;
+        assert a1'(c,|c|-1) == 3;
 
         var d := [-1, 1, 2, -2];
-        var d_ans := [1, 2];
-        assert a1(d) == d_ans;
-
+        assert a1'(d, |d|-1) == 3;
 
         var b := [5,15,-30,10,-5,40,10];
-        var b_ans := [10,-5,40,10];
-        assert a1(b) == b_ans;
+        assert |b| == 7;
+        assert S.seqSum(b[3..]) == 55;
+        assert a1'(b, |b|-1) == 55;
+        */
     }
 }
